hook up bits and pieces to parse all objs in file

main.ml
@@ -4,9 +4,7 @@ open String
 open File
 open IO
 
-open Allparser
-
-let list_of_string s =
+let list_of_string_foo s =
   let rec list_of_string_aux acc s i =
     if i = 0 then
       s.[i]::acc
@@ -15,7 +13,7 @@ let list_of_string s =
   in
     list_of_string_aux [] s (pred (length s));;
 
-let string_of_list l =
+let string_of_list_foo l =
   let s = create (List.length l) in
   let rec string_of_list_aux ll i =
     match ll with
@@ -24,17 +22,21 @@ let string_of_list l =
   in
     string_of_list_aux l 0;;
 
+
+open Allparser
+
+
 let args = Arg.handle [] in
 let infile = open_in (List.at args 0) in
 let data = read_all infile in
 begin
   close_in infile;
-  match main (list_of_string data) with
+  match main (list_of_string_foo data) with
   | SomeE s   -> (* let outfile = open_out (List.at args 1) in
                  begin
-                   nwrite outfile (string_of_list s);
+                   nwrite outfile (string_of_list_foo s);
                    close_out outfile
                  end*)
-                 Print.printf p"%s\n" (string_of_list s)
-  | NoneE err -> Print.printf p"%s\n" (string_of_list err)
+                 Print.printf p"%s\n" (string_of_list_foo s)
+  | NoneE err -> Print.printf p"%s\n" (string_of_list_foo err)
 end
